eve/Src/framework/eiffel2boogie/exec/result/e2b_failed_execution_event.e
@@ -1,0 +1,86 @@
+note
+	description: "Summary description for {E2B_FAILED_EXECUTION_EVENT}."
+	date: "$Date$"
+	revision: "$Revision$"
+
+class
+	E2B_FAILED_EXECUTION_EVENT
+
+inherit
+
+	EVENT_LIST_ITEM_I
+		redefine
+			data
+		end
+
+create
+	make
+
+feature {NONE} -- Initialization
+
+	make (a_data: like data)
+			-- Initialize event item.
+		do
+			data := a_data
+			category := {ENVIRONMENT_CATEGORIES}.none
+			priority := {PRIORITY_LEVELS}.normal
+		ensure
+			data_set: data = a_data
+		end
+
+feature -- Access
+
+	data: STRING
+			-- <Precursor>
+
+	description: STRING_32
+			-- <Precursor>
+		do
+		end
+
+	frozen type: NATURAL_8
+			-- <Precursor>
+		once
+			Result := {EVENT_LIST_ITEM_TYPES}.unknown
+		end
+
+	frozen category: NATURAL_8
+			-- <Precursor>
+
+	frozen priority: INTEGER_8
+			-- <Precursor>
+
+feature -- Status report
+
+	is_invalidated: BOOLEAN
+			-- <Precursor>
+
+	is_valid_data (a_data: ANY): BOOLEAN
+			-- <Precursor>
+		do
+			Result := data /= Void
+		end
+
+feature -- Element change
+
+	set_category (a_category: like category)
+			-- <Precursor>
+		do
+			category := a_category
+		end
+
+	set_priority (a_priority: like priority)
+			-- <Precursor>
+		do
+			priority := a_priority
+		end
+
+feature -- Basic operations
+
+	invalidate
+			-- <Precursor>
+		do
+			is_invalidated := True
+		end
+
+end
